theories/WildCat/Equiv.v
@@ -151,33 +151,43 @@ Global Instance symmetric_cate {A} `{HasEquivs A}
   : Symmetric (@CatEquiv A _ _ _ _ _)
   := fun a b f => cate_inv f.
 
-(** Equivalences can be composed. *)
-Definition compose_catie' {A} `{HasEquivs A} {a b c : A}
-  (g : b $-> c) `{!CatIsEquiv g} (f : a $-> b) `{!CatIsEquiv f}
-  : CatIsEquiv (g $o f).
+(** Anything homotopic to an equivalence is an equivalence. This should not be an instance. *)
+Definition cate_homotopic {A} `{HasEquivs A} {a b : A}
+  (f : a $-> b) `{!CatIsEquiv f} {g : a $-> b} (p : f $== g)
+  : CatIsEquiv g.
 Proof.
   snrapply catie_adjointify.
-  - exact ((Build_CatEquiv f)^-1$ $o (Build_CatEquiv g)^-1$).
-  - nrefine (cat_assoc _ _ _ $@ _).
-    refine (_ $@L ((cate_buildequiv_fun f)^$ $@R _ ) $@ _).
-    nrefine (_ $@L cat_assoc_opp _ _ _ $@ _).
-    nrefine (_ $@L (cate_isretr (Build_CatEquiv f) $@R _) $@ _).
-    nrefine (_ $@L cat_idl _ $@ _).
-    refine ((cate_buildequiv_fun g)^$ $@R _ $@ _).
-    nrapply cate_isretr.
-  - nrefine (cat_assoc _ _ _ $@ _).
-    nrefine (_ $@L cat_assoc_opp _ _ _ $@ _).
-    refine (_ $@L (_ $@L (cate_buildequiv_fun g)^$ $@R _) $@ _).
-    nrefine (_ $@L (cate_issect (Build_CatEquiv g) $@R _) $@ _).
-    nrefine (_ $@L cat_idl _ $@ _).
+  - exact (Build_CatEquiv f)^-1$.
+  - refine (p^$ $@R _ $@ _).
+    refine ((cate_buildequiv_fun f)^$ $@R _ $@ _).
+    apply cate_isretr.
+  - refine (_ $@L p^$ $@ _).
     refine (_ $@L (cate_buildequiv_fun f)^$ $@ _).
-    nrapply cate_issect.
+    apply cate_issect.
 Defined.
 
+(** Equivalences can be composed. *)
 Global Instance compose_catie {A} `{HasEquivs A} {a b c : A}
   (g : b $<~> c) (f : a $<~> b)
+  : CatIsEquiv (g $o f).
+Proof.
+  refine (catie_adjointify _ (f^-1$ $o g^-1$) _ _).
+  - refine (cat_assoc _ _ _ $@ _).
+    refine ((_ $@L cat_assoc_opp _ _ _) $@ _).
+    refine ((_ $@L (cate_isretr _ $@R _)) $@ _).
+    refine ((_ $@L cat_idl _) $@ _).
+    apply cate_isretr.
+  - refine (cat_assoc _ _ _ $@ _).
+    refine ((_ $@L cat_assoc_opp _ _ _) $@ _).
+    refine ((_ $@L (cate_issect _ $@R _)) $@ _).
+    refine ((_ $@L cat_idl _) $@ _).
+    apply cate_issect.
+Defined.
+
+Global Instance compose_catie' {A} `{HasEquivs A} {a b c : A}
+  (g : b $-> c) `{!CatIsEquiv g} (f : a $-> b) `{!CatIsEquiv f}
   : CatIsEquiv (g $o f)
-  := compose_catie' g f.
+  := cate_homotopic _ (cate_buildequiv_fun _ $@@ cate_buildequiv_fun _).
 
 Definition compose_cate {A} `{HasEquivs A} {a b c : A}
   (g : b $<~> c) (f : a $<~> b) : a $<~> c
@@ -335,9 +345,7 @@ Definition cate_inv_compose {A} `{HasEquivs A} {a b c : A} (e : a $<~> b) (f : b
   : cate_fun (f $oE e)^-1$ $== cate_fun (e^-1$ $oE f^-1$).
 Proof.
   refine (_ $@ (compose_cate_fun _ _)^$).
-  nrefine (cate_inv_adjointify _ _ _ _ $@ _).
-  nrefine (cate_inv2 (cate_buildequiv_fun _) $@R _ $@ _).
-  exact (_ $@L cate_inv2 (cate_buildequiv_fun _)).
+  apply cate_inv_adjointify.
 Defined.
 
 Definition cate_inv_V {A} `{HasEquivs A} {a b : A} (e : a $<~> b)
